Update and add examples

Examples.v
@@ -104,11 +104,11 @@ Definition f_psi (x': Proc.t) :=
 
 (* Contract of pre and post condition of procedure f *)
 
-Definition f_pre: assertion := fun s =>
+Definition f_pre: precondition := fun s =>
    s(X2) = (s(X3)) * (s(X4) - s(X1)) /\
    0 <= (s(X1)) /\ Nat.le (s(X1)) (s(X4)).
 
-Definition f_post: assertion := fun s =>
+Definition f_post: postcondition := fun s _ =>
   s(X2) = (s(X3)) * (s(X4)).
 
 (* Contract environment *)
@@ -124,10 +124,9 @@ Definition com_1 := <[
   call(f)
 ]>.
 
-Example hoare_triple_mult: hoare_triple (fun _ => True)
-                              (fun m => f_post m) com_1 f_psi.
+Example hoare_triple_mult: hoare_triple (fun _ => True) f_post com_1 f_psi.
 Proof.
-apply correct with f_phi.
+apply correct with (cl:=f_phi) (l:=[]).
 (* Verification of proof obligation for procedure*)
 * unfold f_psi, f_phi.
   apply Vcg_Opt.tc_p_same.
@@ -176,9 +175,8 @@ apply correct with f_phi.
          unfold f_pre in H.
          decompose [and] H;clear H.
          lia.
-  + split.
-    - auto.
-    - simpl. intros. unfold empty_postcondition. auto.
+  + intros. simpl in H. unfold empty_precondition in H.
+    contradiction.
 * unfold f_psi, f_phi.
   (* Verification of auxilliary proof obligation for command com*)
   intros. apply Vcg_Opt.tc'_same.
@@ -213,62 +211,66 @@ Qed.
 (** Some ltac to automatize the extraction of proof obligation from the list construct
     in relational property verification **)
 
-Ltac ltc3 hy :=
-  inversion hy as [H1];
-  symmetry in H1;
-  apply length_zero_iff_nil in H1;
-  subst.
+Ltac ltc2 phi ps hy hyh:=
+        destruct (mk_rtc'_def _ _ (phi_call (extract phi) ps) _ _ _ _ hy hyh)
+           as (hyr1  & hyr2 & HYP);
+        rewrite HYP;
+        clear HYP hy hyh;
+        rename hyr1 into hy;
+        rename hyr2 into hyh.
 
-Ltac ltc2 phi hy :=
-         destruct (mk_rtc'_def _ _ phi _ _ hy) as (hyr & HYP);
-         rewrite HYP;
-         clear HYP hy;
-         rename hyr into hy.
-
-Ltac ltc7 phi hy H:=
-  ltc2 phi hy;
-  split;[clear hy; inversion H; clear H; apply Vcg_Opt.tc'_same
-        | first [ ltc7 phi hy H| simpl;auto]].
-
-Ltac ltc1 phi hy ml H :=
+Ltac ltc7 phi ps hy hyh H:=
+  ltc2 phi ps hy hyh;
+  split; [ clear hy hyh; simpl H; apply Vcg_Opt.tc'_same
+         | first [ltc7 phi ps hy hyh H | simpl;auto] ].
+  
+Ltac ltc1 phi ps hy hyh ml H :=
          destruct ml;
-         [ discriminate hy
-         | first [ltc3 hy; ltc7 phi hy H| ltc1 phi hy ml H]
+         [ first [ discriminate hy | first [ltc7 phi ps hy hyh H | simpl;auto] ]
+         | first [ discriminate hy | ltc1 phi ps hy hyh ml H ]
          ].
 
-Ltac ltc6 phi hy :=
-       destruct (mk_rtc_def _ _ phi _ _ hy) as (hyr & HYP);
+Ltac ltc6 phi ps hy hyh :=
+       destruct (mk_rtc_def _ _ (phi_call (extract phi) ps) _ _ _ _ hy hyh) 
+           as (hyr1 & hyr2 & HYP);
        rewrite HYP;
-       clear HYP hy;
-       rename hyr into hy.
+       clear HYP hy hyh;
+       rename hyr1 into hy;
+       rename hyr2 into hyh.
 
-Ltac ltc5 phi hy :=
-    intro;
-    intros H1;
-    tryif ltc6 Phi.empty_phi hy;
-          eapply consequence_tc_suite;
-          [ clear H1; ltc5 phi hy | apply Vcg_Opt.tc_same; apply H1]
-    then auto
+Ltac ltc3 phi ps hy hyh:=
+    intro; intro; intros H1; 
+    tryif ltc6 phi ps hy hyh
+    then 
+    eapply consequence_tc_suite;
+    [ clear H1; ltc3 phi ps hy hyh
+    | apply Vcg_Opt.tc_same; apply H1 ]
     else simpl; apply H1.
 
-Ltac ltc4 ml hy phi:=
-         destruct ml;
-         [ discriminate hy
-         | first [ltc3 hy;
-                  ltc6 Phi.empty_phi hy;
-                  eapply consequence_tc_suite;[ ltc5 phi hy | apply Vcg_Opt.tc_same]
-                 | ltc4 ml hy phi]
-          ].
+Ltac ltc5 phi ps hy hyh :=
+    ltc6 phi ps hy hyh;
+    eapply consequence_tc_suite;
+    [ ltc3 phi ps hy hyh
+    | apply Vcg_Opt.tc_same].
 
-Ltac ltc0 phi := apply rcorrect with phi;
+Ltac ltc4 ml hy hyh phi ps :=
+         destruct ml;
+         [ first [ discriminate hy | first [ltc5 phi ps hy hyh | simpl; auto] ]
+         | first [ discriminate hy | ltc4 ml hy hyh phi ps ]
+         ].
+
+Ltac ltc0 phi l hyh := apply rcorrect 
+                with (rcl:=phi) (h:=l) (hyh:=hyh);
                  [
-                 | intros ml hy H;
-                   ltc1 phi hy ml H
-                 | intros ml hy H;
-                   ltc4 ml hy phi;
-                   clear hy;
-                   inversion H;
-                   clear H
+                 | intros ps;
+                   split;
+                   [ intros ml hy H Hr;
+                     ltc1 phi ps hy hyh ml H
+                   | intros ml hy H Hr;
+                     ltc4 ml hy hyh phi ps;
+                     clear hy hyh;
+                     simpl in H
+                   ]
                 ].
 
 (** Examples of proofs of Relational Properties
@@ -290,7 +292,7 @@ Definition swap_2: com := <[ °X1 := °X1 + °X2;
 
 (* Defintion of relational pre and post condition *)
 
-Definition rela_pre (l : list Sigma.sigma) : Prop :=
+Definition rela_pre : r_precondition := fun l =>
   match l with
   | (m1 :: m2 :: []) => m1 (m1 X1) = m2 (m2 X1) /\ m1 (m1 X2) = m2 (m2 X2) /\
                          m1 X1 > 3 /\ m1 X2 > 3 /\ m2 X1 > 3 /\ m2 X2 > 3 /\
@@ -298,7 +300,7 @@ Definition rela_pre (l : list Sigma.sigma) : Prop :=
   | _ => False
   end.
 
-Definition rela_post (l : list Sigma.sigma) : Prop :=
+Definition rela_post : r_postcondition := fun l _ =>
   match l with
   | (m1 :: m2 :: []) => m1 (m1 X1) = m2 (m2 X1) /\ m1 (m1 X2) = m2 (m2 X2)
   | _ => False
@@ -308,9 +310,12 @@ Example relation_swap : relational_prop
                             rela_pre rela_post
                             (swap_1 :: swap_2 :: []) Psi.empty_psi.
 Proof.
-ltc0 Phi.empty_phi.
+assert (hyh :length (swap_1 :: swap_2 :: []) = 
+             length (empty_history:: empty_history :: [])).
+{  simpl. reflexivity. }
+ltc0 R_Phi.empty_r_phi (empty_history :: empty_history :: []) hyh.
 (* Verification of proof obligation for procedure*)
-+ apply tc_p_empty_psi.
++ apply rtc_p_empty_psi.
 (* Verification of auxilliary proof obligation *)
 + simpl. auto.
 + simpl. auto.
@@ -319,132 +324,132 @@ ltc0 Phi.empty_phi.
   intros.
   unfold X1, X2, X3 in *.
   decompose [and] H;clear H.
-  decompose [and] H2;clear H2.
+  decompose [and] H0;clear H0.
   decompose [and] H1;clear H1.
   split.
   * (*<1>*)
-    rewrite H6.
+    rewrite H12.
     mem_d_in m''0 (m''0 2) 1 (m''0 3).
     mem_d_in m''0 (m''0 2) (m''0 1) (m''0 3).
-    rewrite H5.
+    rewrite H11.
     mem_d_in m'' (m'' 1) 1 (m'' (m'' 2)).
     mem_s m'' (m'' 1) (m'' 1) (m'' (m'' 2)).
-    rewrite H3.
+    rewrite H.
     mem_d s 3 2 (s (s 1)).
     mem_d s 3 (s 2) (s (s 1)).
     (*<2>*)
-    rewrite H8.
+    rewrite H14.
     mem_d_in m''2 (m''2 1) 1 (m''2 (m''2 1) - m''2 (m''2 2)).
     mem_s m''2 (m''2 1) (m''2 1) (m''2 (m''2 1) - m''2 (m''2 2)).
-    rewrite H7.
+    rewrite H13.
     mem_d_in m''1 (m''1 2) 2 (m''1 (m''1 1) - m''1 (m''1 2)).
     mem_d_in m''1 (m''1 2) 1 (m''1 (m''1 1) - m''1 (m''1 2)).
     mem_s m''1 (m''1 2) (m''1 2) (m''1 (m''1 1) - m''1 (m''1 2)).
     mem_d_in m''1 (m''1 2) (m''1 1) (m''1 (m''1 1) - m''1 (m''1 2)).
-    rewrite H.
+    rewrite H0.
     mem_d s0 (s0 1) 2 (s0 (s0 1) + s0 (s0 2)).
     mem_d s0 (s0 1) (s0 2) (s0 (s0 1) + s0 (s0 2)).
     mem_d s0 (s0 1) 1 (s0 (s0 1) + s0 (s0 2)).
     mem_s s0 (s0 1) (s0 1) (s0 (s0 1) + s0 (s0 2)).
     - lia.
     (* all the little things *)
-    - rewrite H.
+    - rewrite H0.
       mem_d s0 (s0 1) 1 (s0 (s0 1) + s0 (s0 2)).
       mem_d s0 (s0 1) 2 (s0 (s0 1) + s0 (s0 2)).
       lia.
-    - rewrite H.
+    - rewrite H0.
       mem_d s0 (s0 1) 2 (s0 (s0 1) + s0 (s0 2)).
       lia.
-    - rewrite H.
+    - rewrite H0.
       mem_d s0 (s0 1) 2 (s0 (s0 1) + s0 (s0 2)).
       lia.
-    - rewrite H7.
+    - rewrite H13.
       mem_d_in m''1 (m''1 2) 1 (m''1 (m''1 1) - m''1 (m''1 2)).
-      rewrite H.
+      rewrite H0.
       mem_d s0 (s0 1) 1 (s0 (s0 1) + s0 (s0 2)).
       lia.
-      rewrite H.
+      rewrite H0.
       mem_d s0 (s0 1) 2 (s0 (s0 1) + s0 (s0 2)).
       lia.
-    - rewrite H3.
+    - rewrite H.
       mem_d s 3 1 (s (s 1)).
       lia.
-    - rewrite H5.
+    - rewrite H11.
       mem_d_in m'' (m'' 1) 1 (m'' (m'' 2)).
       mem_d_in m'' (m'' 1) 2 (m'' (m'' 2)).
-      rewrite H3.
+      rewrite H.
       mem_d s 3 1 (s (s 1)).
       mem_d s 3 2 (s (s 1)).
       lia.
-      rewrite H3.
+      rewrite H.
       mem_d s 3 1 (s (s 1)).
       lia.
-      rewrite H3.
+      rewrite H.
       mem_d s 3 1 (s (s 1)).
       lia.
-   - rewrite H5.
+    - rewrite H11.
       mem_d_in m'' (m'' 1) 2 (m'' (m'' 2)).
-      rewrite H3.
+      rewrite H.
       mem_d s 3 2 (s (s 1)).
       lia.
-      rewrite H3.
+      rewrite H.
       mem_d s 3 1 (s (s 1)).
       lia.
  * (*<1>*)
-    rewrite H6.
+    rewrite H12.
     mem_d_in m''0 (m''0 2) 2 (m''0 3).
     mem_s m''0 (m''0 2) (m''0 2) (m''0 3).
-    rewrite H5.
+    rewrite H11.
     mem_d_in m'' (m'' 1) 3 (m'' (m'' 2)).
-    rewrite H3.
+    rewrite H.
     mem_s s 3 3 (s (s 1)).
     (*<2>*)
-    rewrite H8.
+    rewrite H14.
     mem_d_in m''2 (m''2 1) 2 (m''2 (m''2 1) - m''2 (m''2 2)).
     mem_d_in m''2 (m''2 1) (m''2 2) (m''2 (m''2 1) - m''2 (m''2 2)).
-    rewrite H7.
+    rewrite H13.
     mem_d_in m''1 (m''1 2) 2 (m''1 (m''1 1) - m''1 (m''1 2)).
     mem_s m''1 (m''1 2) (m''1 2)  (m''1 (m''1 1) - m''1 (m''1 2)).
-    rewrite H.
+    rewrite H0.
     mem_d s0 (s0 1) 2 (s0 (s0 1) + s0 (s0 2)).
     mem_d s0 (s0 1) (s0 2) (s0 (s0 1) + s0 (s0 2)).
     mem_d s0 (s0 1) 1 (s0 (s0 1) + s0 (s0 2)).
     mem_s s0 (s0 1) (s0 1) (s0 (s0 1) + s0 (s0 2)).
     - lia.
       (* all the little things*)
-    - rewrite H.
+    - rewrite H0.
       mem_d s0 (s0 1) 2 (s0 (s0 1) + s0 (s0 2)).
       lia.
-    - rewrite H7.
+    - rewrite H13.
       mem_d_in m''1 (m''1 2) 1 (m''1 (m''1 1) - m''1 (m''1 2)).
       mem_d_in m''1 (m''1 2) 2 (m''1 (m''1 1) - m''1 (m''1 2)).
-      rewrite H.
+      rewrite H0.
       mem_d s0 (s0 1) 1 (s0 (s0 1) + s0 (s0 2)).
       mem_d s0 (s0 1) 2 (s0 (s0 1) + s0 (s0 2)).
       lia.
-      rewrite H.
+      rewrite H0.
       mem_d s0 (s0 1) 2 (s0 (s0 1) + s0 (s0 2)).
       lia.
-      rewrite H.
+      rewrite H0.
       mem_d s0 (s0 1) 2 (s0 (s0 1) + s0 (s0 2)).
       lia.
-    - rewrite H7.
+    - rewrite H13.
       mem_d_in m''1 (m''1 2) 1 (m''1 (m''1 1) - m''1 (m''1 2)).
-      rewrite H.
+      rewrite H0.
       mem_d s0 (s0 1) 1 (s0 (s0 1) + s0 (s0 2)).
       lia.
-      rewrite H.
+      rewrite H0.
       mem_d s0 (s0 1) 2 (s0 (s0 1) + s0 (s0 2)).
       lia.
-    - rewrite H3.
+    - rewrite H.
       mem_d s 3 1 (s (s 1)).
       lia.
-    - rewrite H5.
+    - rewrite H11.
       mem_d_in m'' (m'' 1) 2 (m'' (m'' 2)).
-      rewrite H3.
+      rewrite H.
       mem_d s 3 2 (s (s 1)).
       lia.
-      rewrite H3.
+      rewrite H.
       mem_d s 3 1 (s (s 1)).
       lia.
 Qed.
@@ -464,13 +469,13 @@ Definition comp: com := <[ if X1 <= X2 && ~ X1 = X2 then
 
 (* Defintion of relational pre and post condition *)
 
-Definition rela_pre_comp (l : list Sigma.sigma) : Prop :=
+Definition rela_pre_comp : r_precondition := fun l =>
   match l with
   | (m1 :: m2 :: []) => m1 X1 = m2 X2 /\ m1 X2 = m2 X1
   | _ => False
   end.
 
-Definition rela_post_comp (l : list Sigma.sigma) : Prop :=
+Definition rela_post_comp : r_postcondition := fun l _ =>
   match l with
   | (m1 :: m2 :: []) => m1 ret + (m2 ret) = 2
   | _ => False
@@ -480,34 +485,36 @@ Example relation_comp : relational_prop
                             rela_pre_comp rela_post_comp
                             (comp :: comp :: []) Psi.empty_psi.
 Proof.
-ltc0 Phi.empty_phi.
+assert (hyh :length (comp :: comp :: []) = 
+             length (empty_history:: empty_history :: [])).
+{  simpl. reflexivity. }
+ltc0 R_Phi.empty_r_phi (empty_history :: empty_history :: []) hyh.
 (* Verification of proof obligation for procedure*)
-+ apply tc_p_empty_psi.
++ apply rtc_p_empty_psi.
 (* Verification of auxilliary proof obligation *)
 + simpl. auto.
 + simpl. auto.
 (* Main proof obligation *)
 + simpl.
   intros.
-  destruct H.
   destruct H0.
-  -- destruct H2.
+  -- destruct H1.
      ** subst. lia.
-     ** destruct H2.
+     ** destruct H3.
         +++ subst.
             mem_s s ret ret 0.
             mem_s s0 ret ret 2.
             reflexivity.
         +++ subst. lia.
-  -- destruct H2.
-     ** destruct H3.
+  -- destruct H1.
+     ** destruct H2.
         +++ subst.
             mem_s s ret ret 2.
             mem_s s0 ret ret 0.
             reflexivity.
         +++ subst. lia.
-     ** destruct H4.
-        +++  subst. lia.
+     ** destruct H2.
+        +++ subst. lia.
         +++ destruct H3.
            *** subst. lia.
            *** subst.
@@ -515,3 +522,164 @@ ltc0 Phi.empty_phi.
                mem_s s0 ret ret 1.
                reflexivity.
 Qed.
+
+(* Example 3 *)
+
+(** Examples of proofs of relational properties using relational contract **)
+
+Parameter f2 : Proc.t.
+
+(* Procedure environment *)
+
+Definition f2_psi (x': Proc.t) :=
+        if Proc.eqb x' f2 then  <[ X1 := X1 + 1 ]> else Psi.empty_psi x'.
+
+(* Definition of relational contract for procedure f *)
+
+Definition f2_r_pre : r_precondition := fun l =>
+  match l with
+  | (m1 :: m2 :: []) => m1 X1 < m2 X1
+  | _ => False
+  end.
+
+Definition f2_r_post : r_postcondition := fun l _ =>
+  match l with
+  | (m1 :: m2 :: []) => m1 X1 < m2 X1
+  | _ => False
+  end.
+
+(* Definition of standard contract for procedure f *)
+
+Definition f2_pre : r_precondition := fun l =>
+  match l with
+  | (m :: []) => True
+  | _ => False
+  end.
+
+Definition f2_post : r_postcondition := fun l _ =>
+  match l with
+  | (m1 :: []) => True
+  | _ => False
+  end.
+
+
+(* Relational contract environment *)
+
+Scheme Equality for list.
+
+Definition f_r_phi (x': list Proc.t) :=
+        if (list_beq  Proc.t) Proc.eqb x' (f2 :: f2 :: []) 
+        then (f2_r_pre,f2_r_post) 
+        else
+            if (list_beq  Proc.t) Proc.eqb x' (f2 :: []) 
+            then (f2_pre,f2_post) 
+            else R_Phi.empty_r_phi x'.
+
+(** Relation Propery **)
+
+Example relation_mono : relational_prop
+                  f2_r_pre f2_r_post
+                  (<[ call(f2) ]> :: <[ call(f2) ]> :: []) f2_psi.
+Proof.
+assert (hyh :length (<[ call(f2) ]>:: <[ call(f2) ]> :: []) = 
+             length (empty_history:: empty_history :: [])).
+{  simpl. reflexivity. }
+ltc0 f_r_phi (empty_history :: empty_history :: []) hyh.
+(* Verification of proof obligation for procedure *)
++ unfold rtc_p.
+  intros.
+  destruct (list_beq Proc.t Proc.eqb f0 [f2; f2]) eqn: E1.
+   (* Proof oblication for relational property {f2_r_pre} f2 ~ f2 {f2_r_post} *)
+    - apply internal_list_dec_bl in E1 ;[ | apply Proc.eqb_eq ].
+      subst.
+      destruct m;[ discriminate hy1 | ].
+      destruct m;[ discriminate hy1 | ].
+      destruct m;[ | discriminate hy1 ].
+      split.
+       (* Verification of auxilliary proof obligation *)
+       * simpl.
+         unfold f2_psi.
+         rewrite Proc.eqb_refl.
+         simpl.
+         auto.
+       (* Main proof obligation *)
+       * simpl.
+         unfold f2_psi, f_r_phi.
+         simpl.
+         rewrite Proc.eqb_refl.
+         simpl.
+         intros.
+         subst.
+         mem_s s X1 X1 (s X1 + 1).
+         mem_s s0 X1 X1 (s0 X1 + 1).
+         simpl in H.
+         apply plus_lt_compat_r.
+         unfold f_r_phi in H.
+         simpl in H.
+         rewrite Proc.eqb_refl in H.
+         simpl in H.
+         assumption.
+   (* Verification of proof obligation for procedure f2*)
+    - destruct (list_beq Proc.t Proc.eqb f0 [f2]) eqn: E2.
+        * apply internal_list_dec_bl in E2 ;[ | apply Proc.eqb_eq ].
+          subst.
+          destruct m;[ discriminate hy1 | ].
+          destruct m;[ | discriminate hy1 ].
+          split.
+          (* Verification of auxilliary proof obligation *)
+          ** simpl.
+             unfold f2_psi.
+             rewrite Proc.eqb_refl.
+             simpl.
+             auto.
+          (* Main proof obligation *)
+          ** simpl.
+             unfold f2_psi, f_r_phi.
+             simpl.
+             rewrite Proc.eqb_refl.
+             simpl.
+             intros.
+             auto.
+         * unfold f_r_phi in H.
+           rewrite E1 in H.
+           rewrite E2 in H.
+           simpl in H.
+           unfold empty_r_precondition in H.
+           contradiction.
+(* Proof obligation for relational property 
+      {f2_r_pre} <[ call(f2) ]> ~ <[ call(f2) ]> {f2_r_post} 
+*)
+(* Verification of auxilliary proof obligation *)
++ simpl. unfold f_r_phi. simpl.
+  rewrite Bool.andb_false_r.
+  rewrite Proc.eqb_refl.
+  simpl.
+  auto.
++ simpl. unfold f_r_phi. simpl.
+  rewrite Bool.andb_false_r.
+  rewrite Proc.eqb_refl.
+  simpl.
+  auto.
+(* Main proof obligation *)
++ simpl.
+  intros.
+  specialize (Hr (f2 :: f2 :: [])).
+  unfold f_r_phi in Hr.
+  replace (list_beq Proc.t Proc.eqb [f2; f2] [f2; f2]) with true in Hr.
+  - specialize (Hr (s :: s0 :: []) (m' :: m'0 :: [])).
+    simpl in Hr.
+    apply Hr.
+    all: try Lia.lia.
+    split. apply H0.
+    split. apply H1.
+    auto.
+  - simpl.
+    symmetry.
+    eapply Bool.andb_true_iff.
+    split.
+    apply Proc.eqb_eq. reflexivity.
+    eapply Bool.andb_true_iff.
+    split.
+    apply Proc.eqb_eq. reflexivity.
+    auto.
+ Qed. 
